(* Copyright Amazon.com, Inc. or its affiliates. All Rights Reserved.
   SPDX-License-Identifier: MIT *)

(*<*)
theory Bool_Type_Lemmas
  imports Core_Expression_Lemmas Bool_Type
begin
(*>*)

lemma evaluate_trueE [micro_rust_elims]:
  assumes \<open>evaluate Bool_Type.true \<sigma> = k\<close>
      and \<open>k = Success True \<sigma> \<Longrightarrow> R\<close>
    shows \<open>R\<close>
using assms by (unfold true_def; elim evaluate_literalE; force)

lemma evaluate_true [micro_rust_simps]:
  shows \<open>evaluate Bool_Type.true \<sigma> = Success True \<sigma>\<close>
by (auto simp add: true_def micro_rust_simps)

lemma evaluate_false [micro_rust_simps]:
  shows \<open>evaluate Bool_Type.false \<sigma> = Success False \<sigma>\<close>
by (auto simp add: false_def micro_rust_simps)

lemma evaluate_falseE [micro_rust_elims]:
  assumes \<open>evaluate Bool_Type.false \<sigma> = k\<close>
      and \<open>k = Success False \<sigma> \<Longrightarrow> R\<close>
    shows \<open>R\<close>
using assms by (unfold false_def; elim evaluate_literalE; force)

lemma evaluate_two_armed_conditionalI [micro_rust_intros]:
    fixes test :: \<open>('s, bool, 'r, 'abort, 'i, 'o) expression\<close>
  assumes \<open>\<And>\<sigma>'. evaluate test \<sigma> = Success True \<sigma>' \<Longrightarrow> k = evaluate t \<sigma>'\<close>
      and \<open>\<And>\<sigma>'. evaluate test \<sigma> = Success False \<sigma>' \<Longrightarrow> k = evaluate f \<sigma>'\<close>
      and \<open>\<And>r \<sigma>'. evaluate test \<sigma> = Return r \<sigma>' \<Longrightarrow> k = Return r \<sigma>'\<close>
      and \<open>\<And>a \<sigma>'. evaluate test \<sigma> = Abort a \<sigma>' \<Longrightarrow> k = Abort a \<sigma>'\<close>
      and \<open>\<And>\<pi> \<sigma>' test'. evaluate test \<sigma> = Yield \<pi> \<sigma>' test' \<Longrightarrow> k = Yield \<pi> \<sigma>' (\<lambda>\<omega>. if (test' \<omega>) \<lbrace> t \<rbrace> else \<lbrace> f \<rbrace>)\<close>
    shows \<open>evaluate (if test \<lbrace> t \<rbrace> else \<lbrace> f \<rbrace>) \<sigma> = k\<close>
using assms by (simp add: two_armed_conditional_def; cases \<open>evaluate test \<sigma>\<close>; intro evaluate_bindI; auto)
 
lemma evaluate_two_armed_conditionalE [micro_rust_elims]:
  assumes \<open>evaluate (two_armed_conditional test t f) \<sigma> = k\<close>
    and \<open>\<And>q \<sigma>' \<sigma>''. evaluate test \<sigma> = Success True \<sigma>' \<Longrightarrow> evaluate t \<sigma>' = k \<Longrightarrow> R\<close>
    and \<open>\<And>q \<sigma>' \<sigma>''. evaluate test \<sigma> = Success False \<sigma>' \<Longrightarrow> evaluate f \<sigma>' = k \<Longrightarrow> R\<close>
    and \<open>\<And>r \<sigma>'. evaluate test \<sigma> = Return r \<sigma>' \<Longrightarrow> k = Return r \<sigma>' \<Longrightarrow> R\<close>
    and \<open>\<And>a \<sigma>'. evaluate test \<sigma> = Abort a \<sigma>' \<Longrightarrow> k = Abort a \<sigma>' \<Longrightarrow>  R\<close>
    and \<open>\<And>\<pi> \<sigma>' test'. evaluate test \<sigma> = Yield \<pi> \<sigma>' test' \<Longrightarrow> 
      k = Yield \<pi> \<sigma>' (\<lambda>\<omega>. if (test' \<omega>) \<lbrace> t \<rbrace> else \<lbrace> f \<rbrace>) \<Longrightarrow> R\<close>
  shows \<open>R\<close>
  using assms by (unfold two_armed_conditional_def) (elim evaluate_bindE; clarsimp split: if_splits)

text\<open>Note that conditionals satisfy some "obvious" properties.  For example, testing against the
\<^emph>\<open>truth\<close> and \<^emph>\<open>falsity\<close> constants collapses the conditional, as one would expect:\<close>
lemma two_armed_conditional_true_false_collapse [micro_rust_simps]:
  shows \<open>\<lbrakk> if True  { \<epsilon>\<open>e\<close> } else { \<epsilon>\<open>f\<close> } \<rbrakk> = e\<close>
    and \<open>\<lbrakk> if False { \<epsilon>\<open>e\<close> } else { \<epsilon>\<open>f\<close> } \<rbrakk> = f\<close>
  by (auto simp add: two_armed_conditional_def true_def false_def micro_rust_simps)

text\<open>Moreover, we can also perform some common-subexpression elimination, by "hoisting" common
expressions that appear in both branches of the conditional out, as follows:\<close>
lemma two_armed_conditional_sequence_hoist [micro_rust_simps]:
  shows \<open>\<lbrakk> if \<epsilon>\<open>c\<close> {
             \<epsilon>\<open>e\<close>;
             \<epsilon>\<open>g\<close>
           } else {
             \<epsilon>\<open>f\<close>;
             \<epsilon>\<open>g\<close> }
         \<rbrakk> = \<lbrakk>
           if \<epsilon>\<open>c\<close> {
             \<epsilon>\<open>e\<close>
           } else {
             \<epsilon>\<open>f\<close>
           };
           \<epsilon>\<open>g\<close>
        \<rbrakk>\<close> (is \<open>?LHS = ?RHS\<close>)
proof -
  have X: \<open>\<And>v e f g. (if v then (e; g) else (f; g)) = (if v then (e; g) else (f; g))\<close>
    by (case_tac v; auto)
  have \<open>?RHS = (let v = c; ((if v then e else f); g))\<close>
    by (simp add: two_armed_conditional_def Core_Expression_Lemmas.bind_assoc sequence_def)  
  also have \<open>... = (let v = c; (if v then (e; g) else (f; g)))\<close>
    by (metis (mono_tags, lifting))
  also have \<open>... = ?LHS\<close>
    by (simp add: two_armed_conditional_def)
  finally show ?thesis by auto
qed

text\<open>Interestingly, this floating out of common subexpressions does not work in the other direction,
nor is it true that we can collapse a conditional where both branches contain the same expression,
\<^term>\<open>e\<close>, to that expression.  This is because the test expression of a conditional may panic, or
return early from a function!\<close>

lemma evaluate_assert_valE [micro_rust_elims]:
  assumes \<open>evaluate (assert_val v) \<sigma> = k\<close>
    and \<open>v = True \<Longrightarrow> k = Success () \<sigma> \<Longrightarrow> R\<close>
    and \<open>v = False \<Longrightarrow> k = Abort AssertionFailed \<sigma> \<Longrightarrow> R\<close>
  shows \<open>R\<close>
  using assms by (cases v; simp add: assert_val_def micro_rust_simps)

lemma evaluate_assertE [micro_rust_elims]:
  assumes \<open>evaluate (assert e) \<sigma> = k\<close>
    and \<open>\<And>\<sigma>'. evaluate e \<sigma> = Success True \<sigma>' \<Longrightarrow> k = Success () \<sigma>' \<Longrightarrow>  R\<close>
    and \<open>\<And>\<sigma>'. evaluate e \<sigma> = Success False \<sigma>' \<Longrightarrow> k = Abort AssertionFailed \<sigma>' \<Longrightarrow> R\<close>
    and \<open>\<And>a \<sigma>'. evaluate e \<sigma> = Abort a \<sigma>' \<Longrightarrow> k = Abort a \<sigma>' \<Longrightarrow> R\<close>
    and \<open>\<And>r \<sigma>'. evaluate e \<sigma> = Return r \<sigma>' \<Longrightarrow> k = Return r \<sigma>' \<Longrightarrow> R\<close>
    and \<open>\<And>\<pi> \<sigma>' e'. evaluate e \<sigma> = Yield \<pi> \<sigma>' e' \<Longrightarrow> k = Yield \<pi> \<sigma>' (\<lambda>\<omega>. assert (e' \<omega>)) \<Longrightarrow> R\<close>
  shows \<open>R\<close>
  using assms by (simp only: assert_def; elim evaluate_bindE evaluate_assert_valE; auto)

lemma evaluate_assertI [micro_rust_intros]:
  assumes \<open>\<And>\<sigma>'. evaluate e \<sigma> = Success True \<sigma>' \<Longrightarrow> k = Success () \<sigma>'\<close>
      and \<open>\<And>\<sigma>'. evaluate e \<sigma> = Success False \<sigma>' \<Longrightarrow> k = Abort AssertionFailed \<sigma>'\<close>
      and \<open>\<And>a \<sigma>'. evaluate e \<sigma> = Abort a \<sigma>' \<Longrightarrow> k = Abort a \<sigma>'\<close>
      and \<open>\<And>\<pi> \<sigma>' e'. evaluate e \<sigma> = Yield \<pi> \<sigma>' e' \<Longrightarrow> k = Yield \<pi> \<sigma>' (\<lambda>\<omega>. assert (e' \<omega>))\<close>
      and \<open>\<And>r \<sigma>'. evaluate e \<sigma> = Return r \<sigma>' \<Longrightarrow> k = Return r \<sigma>'\<close>
  shows \<open>evaluate (assert e) \<sigma> = k\<close>
  using assms
  by (auto intro: evaluate_bindI simp add: assert_def assert_val_def micro_rust_simps)

text\<open>In degenerate cases, this assertion expression behaves like a form of \<^term>\<open>panic\<close>:\<close>
lemma assert_false_sequence [micro_rust_simps]:
  shows \<open>(assert (\<up>False); e) = assert (\<up>False)\<close>
  by (simp add: micro_rust_simps assert_def assert_val_def)

text\<open>...and \<^term>\<open>skip\<close>:\<close>
lemma assert_true_sequence [micro_rust_simps]:
  shows \<open>\<lbrakk> assert!(True); \<epsilon>\<open>e\<close> \<rbrakk> = e\<close>
  by (simp add: micro_rust_simps assert_def assert_val_def)

lemma evaluate_negation_literal [micro_rust_simps]:
  shows \<open>\<lbrakk> !c \<rbrakk> = \<lbrakk> \<llangle>\<not>c\<rrangle> \<rbrakk>\<close>
  by (clarsimp simp add: micro_rust_simps negation_def)

lemma evaluate_conjunction_literal [micro_rust_simps]:
  shows \<open>\<lbrakk> c && \<epsilon>\<open>d\<close> \<rbrakk> = \<lbrakk> if c { \<epsilon>\<open>d\<close> } else { False } \<rbrakk>\<close>
  by (clarsimp simp add: micro_rust_simps urust_conj_def two_armed_conditional_def false_def)

lemma evaluate_disjunction_literal [micro_rust_simps]:
  shows \<open>\<lbrakk> c || \<epsilon>\<open>e\<close> \<rbrakk> = \<lbrakk> if c { True } else { \<epsilon>\<open>e\<close> } \<rbrakk>\<close>
  by (clarsimp simp add: micro_rust_simps urust_disj_def two_armed_conditional_def true_def)

lemma evaluate_eq_literal [micro_rust_simps]:
  shows \<open>\<lbrakk> c == d \<rbrakk> = \<lbrakk> \<llangle>c = d\<rrangle> \<rbrakk>\<close>
  by (clarsimp simp add: micro_rust_simps urust_eq_def)

lemma evaluate_neq_literal [micro_rust_simps]:
  shows \<open>\<lbrakk> c != d \<rbrakk> = \<lbrakk> \<llangle>c \<noteq> d\<rrangle> \<rbrakk>\<close>
  by (clarsimp simp add: micro_rust_simps urust_neq_def)

(*<*)
end
(*>*)
